Prove upper bound, one direction

BoltLean/Ltl.lean
@@ -1,10 +1,16 @@
+import BoltLean.Helpers
+
 structure Trace (n_pred: Nat) where
   length: Nat
+  pos_length : length > 0
+  pos_n_pred: n_pred > 0
   predicates : Vector (Vector Bool length) n_pred
 deriving Repr
 
 /-- LTL Formulas in NNF -/
 inductive Formula n_pred
+  | True : Formula n_pred
+  | False : Formula n_pred
   | Var : Fin n_pred -> (neg: Bool) -> Formula n_pred -- neg: Whether the variable is negated
   | Next : Formula n_pred -> Formula n_pred
   | WeakNext : Formula n_pred -> Formula n_pred
@@ -19,8 +25,10 @@ namespace Formula
 
   def eval_aux (phi: Formula n) (t: Trace n) (i: Fin t.length): Prop :=
     match phi with
+    | True => _root_.True
+    | False => _root_.False
     | Var v neg => xor t.predicates[v][i] neg
-    | Next psi => if h: i < t.length - 1 then eval_aux psi t ⟨i.val + 1, by omega⟩ else False
+    | Next psi => if h: i < t.length - 1 then eval_aux psi t ⟨i.val + 1, by omega⟩ else _root_.False
     | WeakNext psi => (h: i < t.length - 1) → eval_aux psi t ⟨i.val + 1, by omega⟩
     | Globally psi => ∀ j, j ≥ i  → eval_aux psi t j
     | Finally psi => ∃ j, j ≥ i ∧ eval_aux psi t j
@@ -31,62 +39,53 @@ namespace Formula
                               (∀ k, i ≤ k → k < j → eval_aux psi1 t k)
 
   def eval (phi : Formula n) (t : Trace n) : Prop :=
-    if h : t.length > 0 then
-      eval_aux phi t ⟨0, h⟩
-    else
-      match phi with
-      -- I guess technically, WeakNext and Globally
-      -- are both true on empty traces, and are the only ones.
-      | WeakNext _ | Globally _ => True
-      | Or psi1 psi2 => eval psi1 t ∨ eval psi2 t
-      | And psi1 psi2 => eval psi1 t ∧ eval psi2 t
-      | _ => False
+    eval_aux phi t ⟨0, t.pos_length⟩
 
 
-  theorem or_eval (phi psi: Formula n) (t: Trace n):
-    (phi.Or psi).eval t ↔ phi.eval t ∨ psi.eval t  := by
-      constructor
-      . intro h
-        simp [eval, eval_aux] at h
-        by_cases htl: 0 < t.length
-        . simp [htl] at h
-          unfold eval
-          simp [htl]
-          exact h
-        . simp [htl] at h
-          assumption
-      . intro h
-        rw [eval]
-        by_cases htl: 0 < t.length
-        all_goals simp [htl]
-        . unfold eval at h
-          simp [htl] at h
-          rw [eval_aux]
-          assumption
-        . exact h
+  -- theorem or_eval (phi psi: Formula n) (t: Trace n):
+  --   (phi.Or psi).eval t ↔ phi.eval t ∨ psi.eval t  := by
+  --     constructor
+  --     . intro h
+  --       simp [eval, eval_aux] at h
+  --       by_cases htl: 0 < t.length
+  --       . simp [htl] at h
+  --         unfold eval
+  --         simp [htl]
+  --         exact h
+  --       . simp [htl] at h
+  --         assumption
+  --     . intro h
+  --       rw [eval]
+  --       by_cases htl: 0 < t.length
+  --       all_goals simp [htl]
+  --       . unfold eval at h
+  --         simp [htl] at h
+  --         rw [eval_aux]
+  --         assumption
+  --       . exact h
 
 
-  theorem and_eval (phi psi: Formula n) (t: Trace n):
-    (phi.And psi).eval t ↔ phi.eval t ∧ psi.eval t  := by
-      constructor
-      . intro h
-        simp [eval, eval_aux] at h
-        by_cases htl: 0 < t.length
-        . simp [htl] at h
-          unfold eval
-          simp [htl]
-          exact h
-        . simp [htl] at h
-          assumption
-      . intro h
-        rw [eval]
-        by_cases htl: 0 < t.length
-        all_goals simp [htl]
-        . unfold eval at h
-          simp [htl] at h
-          rw [eval_aux]
-          assumption
-        . exact h
+  -- theorem and_eval (phi psi: Formula n) (t: Trace n):
+  --   (phi.And psi).eval t ↔ phi.eval t ∧ psi.eval t  := by
+  --     constructor
+  --     . intro h
+  --       simp [eval, eval_aux] at h
+  --       by_cases htl: 0 < t.length
+  --       . simp [htl] at h
+  --         unfold eval
+  --         simp [htl]
+  --         exact h
+  --       . simp [htl] at h
+  --         assumption
+  --     . intro h
+  --       rw [eval]
+  --       by_cases htl: 0 < t.length
+  --       all_goals simp [htl]
+  --       . unfold eval at h
+  --         simp [htl] at h
+  --         rw [eval_aux]
+  --         assumption
+  --       . exact h
 
 
 end Formula
