BoltLean/Domination.lean
@@ -13,12 +13,10 @@ theorem or_dominates (phi psi: Formula n) (f: Formula n):
     simp [eval, eval_aux] at h2
     simp [eval, eval_aux]
     match h2 with
-    | ⟨hi, h_or⟩ => exists hi
-                    match h_or with
-                    | .inl hf => apply Or.inl; assumption
-                    | .inr h_psi => apply Or.inr
-                                    simp [eval, hi] at h1;
-                                    apply h1; assumption
+    | .inl hf => apply Or.inl; assumption
+    | .inr h_psi => apply Or.inr
+                    simp [eval] at h1;
+                    apply h1; assumption
 
 
 end Formula
