BoltLean/UpperBound.lean
@@ -1,0 +1,207 @@
+import BoltLean.Ltl
+
+namespace Trace
+  def get_exact_var (t: Trace n) (i: Fin t.length) (v: Fin n): Formula n :=
+    Formula.Var v (not t.predicates[v][i])
+
+  /-- Auxiliary functions for constructing a formula that is true on t and only on t-/
+  def exact_at_pos (t: Trace n) (i: Fin t.length): Formula n :=
+    let all_indices := List.finRange n
+    let all_var := all_indices.map (t.get_exact_var i)
+    all_var.foldr (fun phi psi => phi.And psi) Formula.True
+
+
+  def subrange (start: Nat) : List (Fin n) :=
+    if h: start < n then
+      ⟨start, by omega⟩ :: subrange (start + 1)
+    else
+      []
+
+  def exact (t: Trace n) : Formula n :=
+    let all_indices := subrange 0
+    let all_exact := all_indices.map t.exact_at_pos
+    -- Ensure that the trace has the right length
+    -- by checking WeakNext False at the end
+    all_exact.foldr (fun phi psi => phi.And psi.WeakNext) Formula.False
+
+  -- Scaffolding for proving that the `exact` construction works:
+  -- - it is true on `t`
+  -- - it is only true on `t`
+  /-- Helper lemma: Proves that the folded AND formula is true for ANY list of variables -/
+  theorem exact_at_pos_eval_aux_list (t: Trace n) (i: Fin t.length) (vars : List (Fin n)):
+    ((vars.map (t.get_exact_var i)).foldr (fun phi psi => phi.And psi) Formula.True).eval_aux t i := by
+    induction vars with
+    | nil => simp [Formula.eval_aux]
+    | cons hd tl ih =>
+      simp [Formula.eval_aux, get_exact_var]
+      exact ih
+
+  /-- Correctness: `t.exact_at_pos i` evaluates to true on `t` at `i` -/
+  theorem exact_at_pos_eval_aux (t: Trace n) (i: Fin t.length):
+    (t.exact_at_pos i).eval_aux t i := by
+    unfold exact_at_pos
+    apply exact_at_pos_eval_aux_list
+
+  /-- Helper lemma: Evaluates the formula suffix starting from an arbitrary time `i` -/
+  theorem exact_eval_suffix (t: Trace n) (rem: Nat) (i: Fin t.length) (h_rem: t.length - i.val = rem) :
+    (((subrange i
+      ).map t.exact_at_pos
+     ).foldr
+        (fun phi psi => phi.And psi.WeakNext)
+        Formula.False
+    ).eval_aux t i := by
+    -- We do induction on the number of remaining steps in the trace
+    induction rem generalizing i with
+    | zero => omega
+    | succ k ih =>
+      unfold subrange
+      by_cases hi: i < t.length
+      . simp [hi]
+        unfold Formula.eval_aux
+        constructor
+        . exact exact_at_pos_eval_aux t i
+        . unfold Formula.eval_aux
+          intro hi
+          apply ih ⟨i.val+1, by omega⟩
+          have hik : t.length - (i.val+1) = k := by omega
+          omega
+      . have he: i.val = t.length -1 := by
+          omega
+        simp [he]
+        omega
+
+  /-- Correctness: `t.exact` evaluates to true on `t` -/
+  theorem exact_eval (t: Trace n) : (t.exact).eval t := by
+    unfold exact
+    unfold Formula.eval
+    have h_rem : t.length - 0 = t.length := by omega
+    have h := exact_eval_suffix t (t.length) ⟨0, t.pos_length⟩ h_rem
+    simp
+    exact h
+
+  -- Soundness
+  theorem diff_exist_diff_var (t t': Trace n) (h: t ≠ t'):
+    t.length ≠ t'.length
+      ∨ exists (i: Fin t.length) (v: Fin n) (h': i < t'.length),
+        t.predicates[v][i] ≠ t'.predicates[v][i] := by
+      by_cases hl: t.length = t'.length
+      . right
+        apply Classical.byContradiction
+        intro h_contra
+        apply h
+        cases t
+        cases t'
+        simp at hl
+        subst hl
+        simp at *
+        apply Vector.ext
+        intro v hv
+        apply Vector.ext
+        intro i hi
+        exact h_contra ⟨i, hi⟩ ⟨v, hv⟩
+      . left
+        exact hl
+
+  -- theorem exact_at_pos_eval_iff
+  --   (t t': Trace n) (i: Fin t.length) (i': Fin t'.length) :
+  --     (t.exact_at_pos i).eval_aux t' i'
+  --       ↔ (∀ (v : Fin n), t.predicates[v][i] = t'.predicates[v][i']) := by
+  --   -- Proof by induction or well-founded recursion on (n - v)
+  --   constructor
+  --   . intro h v
+  --     unfold exact_at_pos at h
+  --     unfold Formula.eval_aux at h
+  --     simp at h
+  --   . sorry
+
+  -- theorem not_eval_aux_exact_at_pos_if_diff_pred (t t': Trace n)
+  --     (i: Fin t.length) (v: Fin n)
+  --     (hi: i < t'.length) (h: t.predicates[v][i] ≠ t'.predicates[v][i]) :
+  --   ¬(t.exact_at_pos i v).eval_aux t' ⟨i.val, hi⟩ := by
+  --  unfold exact_at_pos
+  --  simp
+  --  split
+  --  . next hif =>
+  --                simp [Formula.eval_aux]
+  --                intro he
+  --                simp at h
+  --                rw [eq_comm] at he
+  --                exact absurd he h
+  --  . next hnif => simp [Formula.eval_aux]
+  --                 simp at h
+  --                 rw [eq_comm] at h
+  --                 exact h
+
+  -- theorem not_eval_aux_exact_at_pos_if_diff_pred_lt (t t': Trace n)
+  --     (i: Fin t.length) (v v': Fin n) (hv: v' ≤ v)
+  --     (hi: i < t'.length) (h: t.predicates[v][i] ≠ t'.predicates[v][i]) :
+  --   ¬(t.exact_at_pos i v').eval_aux t' ⟨i.val, hi⟩ := by
+  --   by_cases he: v' = v
+  --   . rw [he]
+  --     apply not_eval_aux_exact_at_pos_if_diff_pred <;> assumption
+  --   . unfold exact_at_pos
+  --     have hv': v' < n-1 := by omega
+  --     simp [hv']
+  --     simp [Formula.eval_aux]
+  --     intro hp
+  --     let v'' := v'.val+1
+  --     have hv'': v'' ≤ v := by omega
+  --     apply not_eval_aux_exact_at_pos_if_diff_pred_lt t t' i v ⟨v'', by omega⟩ hv'' hi h
+
+  -- theorem not_eval_aux_exact_aux_if_diff_pred (t t': Trace n)
+  --     (i: Fin t.length) (v: Fin n)
+  --     (hi: i < t'.length) (h: t.predicates[v][i] ≠ t'.predicates[v][i]) :
+  --   ¬(t.exact_aux i).eval_aux t' ⟨i.val, hi⟩ := by
+  --   unfold exact_aux
+  --   split
+  --   . next hif => simp
+  --                 unfold Formula.eval_aux
+  --                 rw [Classical.not_and_iff_not_or_not]
+  --                 left
+  --                 apply not_eval_aux_exact_at_pos_if_diff_pred_lt
+  --                 all_goals try assumption
+  --                 apply Nat.zero_le
+  --   . next hnif => simp
+  --                  apply not_eval_aux_exact_at_pos_if_diff_pred_lt
+  --                  all_goals try assumption
+  --                  apply Nat.zero_le
+
+
+  -- theorem not_eval_aux_exact_aux_if_diff_pred_lt (t t': Trace n)
+  --     (i i': Fin t.length) (hi': i' ≤ i) (v: Fin n)
+  --     (hi: i < t'.length) (h: t.predicates[v][i] ≠ t'.predicates[v][i]) :
+  --   ¬(t.exact_aux i').eval_aux t' ⟨i'.val,by omega⟩ := by
+  --   by_cases he: i = i'
+  --   . subst he
+  --     apply not_eval_aux_exact_aux_if_diff_pred <;> assumption
+  --   . unfold exact_aux
+  --     simp
+  --     have h1: i' < t.length - 1 := by omega
+  --     simp [h1]
+  --     unfold Formula.eval_aux
+  --     simp
+  --     intro h2
+  --     simp [Formula.eval_aux]
+  --     intro
+  --     apply not_eval_aux_exact_aux_if_diff_pred_lt
+  --     all_goals try assumption
+  --     rw [Nat.ne_iff_lt_or_gt] at he
+  --     sorry
+
+  -- /-- Soundness: `t.exact` only accepts `t`-/
+  -- theorem exact_eval_only (t t': Trace n) (h: t ≠ t'): ¬(t.exact).eval t' := by
+  --   have h1 := diff_exist_diff_var t t' h
+  --   match h1 with
+  --   | Or.inl h2 => sorry
+  --   | Or.inr h2 => match h2 with
+  --     | ⟨i, v, h', hd⟩ => unfold exact
+  --                         unfold Formula.eval
+  --                         apply not_eval_aux_exact_aux_if_diff_pred t t' i
+  --                         assumption
+
+end Trace
+
+-- theorem exact_eval (t: Trace n) :
+--   exists (phi: Formula n), phi.eval t ∧
+--     forall (t': Trace n), t ≠ t' → ¬phi.eval t' := by
+--     sorry
